capabilities/big_step.v
@@ -1,0 +1,279 @@
+Set Warnings "-notation-overridden,-parsing".
+(*
+Author: Rodrigo Raya
+
+Following "The Semantics of Ownership and Borrowing in the Rust Programming Language" by Nienke Wessel.
+*)
+
+From Coq Require Import Bool.Bool.
+From Coq Require Import Init.Nat.
+From Coq Require Import Arith.Arith.
+From Coq Require Import ZArith.Int.
+From Coq Require Import Arith.EqNat.
+From Coq Require Import omega.Omega.
+From Coq Require Import Lists.List.
+From Coq Require Import Strings.String.
+From Coq Require Import Logic.FunctionalExtensionality.
+
+Import ListNotations.
+Open Scope string_scope.
+Open Scope list_scope.
+
+Definition vname := string.
+
+Inductive zext :=
+| non_declared
+| not_assigned
+| val : Z -> zext.
+
+Bind Scope move_scope with zext.
+Notation "-__u" := non_declared : move_scope.
+Notation "⊥" := not_assigned : move_scope.
+ 
+Inductive type :=
+| Int : type.
+
+Inductive expr :=
+| var : vname -> expr
+| integer : Z -> expr
+| add : expr -> expr -> expr.
+
+Inductive com :=
+| Skip : com
+| Seq : com -> com -> com
+| Bind : vname -> type -> com -> com
+| Assign : vname -> expr -> com.
+
+Bind Scope move_scope with com.
+Notation "c1 ;; c2" :=
+  (Seq c1 c2) (at level 60, right associativity) : move_scope.
+(*
+The notation emphasizes that a let statement in Rust:
+
+let x = e
+
+actually refers to a two step process:
+
+1. Variable x is declared.
+2. A value is assigned to the resource x owns.
+
+We instead write:
+
+let x in (x = e) 
+*)
+Notation "'LET' x ',' t 'IN' b" :=
+  (Bind x t b) (at level 50, left associativity) : move_scope.
+Notation "x ';=' e" :=
+  (Assign x e) (at level 50) : move_scope.
+
+Definition prog0 : com := Skip.
+
+(* Some variables to work with *)
+Definition X : string := "x".
+Definition Y : string := "y".
+Definition Z : string := "z".
+
+Definition prog1 : com := LET X , Int IN Skip.
+
+Definition prog2 : com :=
+  LET X , Int IN (X ;= (integer 0) ;;
+   LET Y , Int IN (Y ;= (var X) ;;
+    LET Z , Int IN (Z ;= (var Y)))).
+
+Definition state := vname -> zext.
+
+Definition abs_state (A:Type) := string -> A.
+
+Definition update {abs_value: Type} 
+  (s : abs_state abs_value) (x : string) (v : abs_value) :=
+  fun x' => if string_dec x x' then v else s x'.
+
+Lemma update_eq : forall (s: state) (x: string) (v: zext),
+    update s x v x = v.
+Proof.
+  intros. unfold update. destruct (string_dec x x) as [|Hs].
+  - reflexivity. 
+  - contradiction.
+Qed.
+
+Lemma update_neq : forall (s: state) (x1 x2: string) (v: zext),
+    x1 <> x2 -> update s x1 v x2 = s x2.
+Proof.
+  intros. unfold update. destruct (string_dec x1 x2).
+  - contradiction.
+  - reflexivity.
+Qed.
+
+Definition update_list {abs_value: Type} 
+  (s : abs_state abs_value) (l : list string) (v : abs_value) :=
+  fold_left (fun (s': abs_state abs_value) (x: string)
+             => update s' x v) l s.
+ 
+Fixpoint contains (l: list string) (x: string): bool :=
+  match l with
+  | [] => false
+  | h :: tl => (if (string_dec h x) then true else (contains tl x))
+  end.
+
+(* Some lemmas to finish the last case of variable allocation *)
+Lemma update_comm_elems :
+  forall (l1 l2: string) (s: state)  (x: string) (v: zext),
+    update_list s [l1;l2] v x = update_list s [l2;l1] v x.
+Proof.
+  intros. 
+  simpl.
+  destruct (string_dec l1 l2).
+  - subst. reflexivity.
+  - unfold update.
+    destruct (string_dec l2 x);
+    destruct (string_dec l1 x); try(reflexivity).
+Qed.
+
+Lemma update_comm_list :
+  forall (l1: string) (l2: list string) (s: state)
+    (x: string) (v: zext),
+    update_list s (l1::l2) v x = update_list s (l2++[l1]) v x.
+Proof.
+  induction l2.
+  - simpl. intros. reflexivity.
+  - simpl. intros. rewrite <- (IHl2 (update s a v) x v).
+    simpl.
+    assert (update (update s l1 v) a v =
+            update (update s a v) l1 v).
+    { apply functional_extensionality. intros.
+      apply update_comm_elems. }
+    rewrite H. reflexivity.
+Qed.
+
+Lemma update_comm :
+  forall (l1 l2: list string) (s: state) (x: string) (v: zext),
+    update_list s (l1++l2) v x = update_list s (l2++l1) v x.
+Proof.
+  induction l1.
+  - simpl. intros. rewrite app_nil_r. reflexivity.
+  - intros. simpl.
+    assert (l2 ++ a :: l1 = (l2 ++ [a]) ++ l1).
+    { apply (app_assoc l2 [a] l1). }
+    rewrite H.
+    rewrite <- (IHl1 (l2++[a]) s x v).
+    rewrite app_assoc.
+    rewrite <- (update_comm_list a (l1++l2)).
+    reflexivity.
+Qed.
+
+Lemma update_last:
+  forall (l: list string) (s: state)  (x: string) (v: zext),
+    update_list s (l++[x]) v x = v.
+Proof.
+  induction l.
+  - intros. simpl. apply update_eq.
+  - intros. simpl. apply IHl.
+Qed.
+
+Lemma update_head :
+  forall (l: list string) (s: state)  (x: string) (v: zext),
+     update_list s (x::l) v x = v.
+Proof.
+  intros. 
+  assert(update_list s (x::l) v x = update_list s (l++[x]) v x).
+  { apply update_comm_list. }
+  rewrite H. apply update_last. 
+Qed.
+
+Lemma update_contained :
+  forall (l: list string) (s: state)  (x: string) (v: zext),
+     contains l x = true -> update_list s l v x = v.
+Proof.
+  induction l; intros.   
+  - discriminate.
+  - destruct (string_dec a x).
+    + subst. apply update_head.
+    + simpl. apply IHl. simpl in H.
+      destruct (string_dec a x). contradiction. apply H.      
+Qed.
+
+Lemma update_not_contained :
+  forall (l: list string) (s: state)  (x: string) (v: zext),
+     contains l x = false -> update_list s l v x = s x.
+Proof.
+  induction l; intros.   
+  - reflexivity.
+  - simpl. rewrite (IHl (update s a v) x v).
+    + unfold update. simpl in H. destruct (string_dec a x).
+      ++ discriminate.
+      ++ reflexivity.
+    + simpl in H. destruct (string_dec a x).
+      ++ discriminate.
+      ++ apply H.    
+Qed.
+
+Fixpoint vars (e: expr): list string :=
+  match e with
+  | var vn => [vn]
+  | integer i => []
+  | add e__1 e__2 => vars (e__1) ++ vars(e__2)
+  end.
+
+Fixpoint aval (s : state) (e : expr): zext :=
+  match e with
+  | var vn => s vn
+  | integer i => val i
+  | add e__1 e__2 =>
+     match (aval s e__1, aval s e__2) with
+     | (val i, val j) => val (i + j)
+     | _ => non_declared
+     end
+  end.
+
+Reserved Notation "e '⟹__b' b" (at level 90, left associativity).
+
+Inductive big_step : com * state -> state -> Prop :=
+| BSkip (s: state) : (Skip, s) ⟹__b s
+| BSeq (s__1 s__2 s__3: state) (c__1 c__2: com) :
+    (c__1,s__1) ⟹__b s__2 -> (c__2,s__2) ⟹__b s__3 -> (c__1;;c__2,s__1) ⟹__b s__3
+| BLet (s s': state) (c : com) (x : vname) (t : type) :
+    (c,update s x ⊥) ⟹__b s' ->
+     (LET x , t IN c, s) ⟹__b (update s' x (s x))
+| BAssign (s: state) (e : expr) (x: string) :
+    aval s (var x) = ⊥ -> aval s e <> ⊥ -> aval s e <> -__u ->
+    (x ;= e, s) ⟹__b (update_list (update s x (aval s e)) (vars e) -__u)
+where "e '⟹__b' b" := (big_step e b) : move_scope.
+
+Open Scope move_scope.
+
+Theorem big_step_deterministic : forall (c: com) (s s__1 s__2 : state),
+    (c,s) ⟹__b s__1 -> (c,s) ⟹__b s__2 -> s__1 = s__2.
+Proof.
+  intros c.
+  induction c; intros s s__1 s__2 H1 H2;
+  inversion H1; inversion H2; subst; try(reflexivity).
+  - assert(eq1: s__3 = s__6). { apply (((IHc1 s s__3 s__6) H5) H11). }
+    rewrite <- eq1 in H12.
+    apply (((IHc2 s__3 s__1 s__2) H6) H12). 
+  - rewrite ((IHc (update s v ⊥) s' s'0) H5 H10). reflexivity.
+Qed.
+
+(*
+After execution, a program no longer has variables in memory.
+*)
+Theorem variable_allocation: forall (c: com) (s s' : state) (vn y : string),
+    (c,s) ⟹__b s' -> aval s (var y) = -__u -> aval s' (var y) = -__u.
+Proof.
+  induction c; intros s s' vn y H1 H2; inversion H1; subst.
+  - apply H2.
+  - assert(eq1: aval s__2 (var y) = -__u).
+    { apply ((IHc1 s s__2 vn y) H5 H2). }
+    apply ((IHc2 s__2 s' vn y) H6 eq1).
+  - destruct (string_dec v y); simpl.
+    + rewrite e. rewrite update_eq. apply H2.
+    + rewrite update_neq; try (apply n).
+      apply ((IHc (update s v ⊥) s'0 vn y) H5); simpl.
+      rewrite update_neq; try (apply n). apply H2.
+  - destruct (string_dec v y). 
+    + subst. rewrite H2 in H4. discriminate.
+    + destruct (contains (vars e) y) eqn: H.
+      ++ simpl. apply update_contained. apply H.
+      ++ simpl. rewrite update_not_contained; try(apply H). simpl.
+        unfold update. destruct (string_dec v y);  try(contradiction).
+        apply H2.
+Qed.
