capabilities/moving.v
@@ -1,0 +1,769 @@
+Set Warnings "-notation-overridden,-parsing".
+(*
+Author: Rodrigo Raya
+
+Following "The Semantics of Ownership and Borrowing in the Rust Programming Language" by Nienke Wessel.
+
+Moving means move only
+
+Can only assign variables if you do so ownership of the resource
+is moved to that varaible.
+
+Cannot borrow and nothing is immutable.
+*)
+
+From Coq Require Import Bool.Bool.
+From Coq Require Import Init.Nat.
+From Coq Require Import Arith.Arith.
+From Coq Require Import ZArith.Int.
+From Coq Require Import Arith.EqNat.
+From Coq Require Import omega.Omega.
+From Coq Require Import Lists.List.
+From Coq Require Import Strings.String.
+From Coq Require Import Logic.FunctionalExtensionality.
+(* for specific induction *)
+Require Import Coq.Program.Equality.
+Require Import Capabilities.big_step.
+Require Import Capabilities.small_step.
+
+(*
+We have to check that the small and big step semantics match.
+In particular, there is a side condition of the assignment in 
+the big step semantics that needs to be checked.
+
+We implement this side conditions as compile cheks. 
+ *)
+
+Inductive abstract_zext :=
+| non_declared
+| not_assigned
+| not_specified.
+
+Notation rstate := (string -> abstract_zext).
+
+Bind Scope move_scope with abstract_zext.
+Notation "⊥__a" := non_declared : move_scope.
+Notation "-__a" := not_assigned: move_scope.
+Notation "*__a" := not_specified : move_scope.
+
+Definition related_states (s: state) (r: rstate) :=
+  (forall (x:string),
+      ((s x) = ⊥ <-> (r x) = ⊥__a) /\
+      ((s x) = -__u <-> (r x) = -__a) /\
+      ((exists z, (s x) = val z) <-> (r x) = *__a)).
+
+Reserved Notation "e '⟹__c' b" (at level 90, left associativity).
+
+Inductive ainstruction :=
+| aprog_instr : vname * abstract_zext -> ainstruction
+| acommand : com -> ainstruction.
+
+Definition alist := List.list ainstruction.
+
+Notation "'ac' com" := (acommand com) (at level 20) : move_scope.
+Notation "'ai' p_instr" := (aprog_instr p_instr) (at level 20) : move_scope.
+
+Inductive compile_step :
+  (ainstruction * alist * rstate) + bool ->
+  (ainstruction * alist * rstate) + bool -> Prop :=
+| CSkipNil (r: rstate) :
+    inl (ac Skip, nil, r) ⟹__c inr true
+| CSkipCons (p: ainstruction) (l: alist) (r: rstate):
+    inl (ac Skip, p :: l, r) ⟹__c inl (p, l, r)
+| CSeq (c1 c2: com) (l: alist) (r: rstate):
+    inl (ac (c1;;c2),l,r) ⟹__c inl (ac c1,ac c2 :: l,r)
+| CAss_legal (x: string) (e: expr) (l: alist) (r: rstate):
+    ((r x) = ⊥__a) -> ((forall y, In y (vars e) -> r(y) = *__a)) ->
+    inl (ac (x ;= e),l,r) ⟹__c
+    inl (ac Skip,l, update_list (update r x *__a) (vars e) -__a)
+| CAss_illegal (x: string) (e: expr) (l: alist) (r: rstate):
+    ((r x) <> ⊥__a \/ (exists y, In y (vars e) /\ r(y) <> *__a)) ->
+    inl (ac (x ;= e),l,r) ⟹__c inr false
+| CLet (x: string) (t: type) (c': com) (l: alist) (r: rstate):
+    inl (ac (LET x, t IN c'),l,r) ⟹__c   
+    inl (ac c', (ai (x,r(x))) :: l, update r x ⊥__a)
+| CBind (x: string) (v: abstract_zext) (r: rstate) (l: alist) :
+    inl (ai (x,v),l,r) ⟹__c inl (ac Skip,l,update r x v)
+where "e '⟹__c' b" := (compile_step e b) : move_scope.
+
+Notation "x '⟹__c*' y" := (star compile_step x y) (at level 30) : move_scope.
+
+
+Fixpoint aicommand (c': com) :=
+  match c' with
+  | Skip => 1
+  | (c1 ;; c2) => aicommand c1 + aicommand c2 + 1
+  | (x ;= e) => 2
+  | (LET x , t IN c') => aicommand c' + 3 
+  end. 
+  
+Fixpoint ailength (c': ainstruction) :=
+  match c' with
+  | (ai (x,v)) => 2
+  | (ac c') => aicommand c'
+  end. 
+  
+Fixpoint allength (l: alist) :=
+  match l with
+  | nil => 0
+  | h :: tl => ailength h + allength tl
+  end.
+
+Inductive terminating {A} (r: A -> A -> Prop) (c': A): Prop :=
+| TStep : (forall c1, r c' c1 -> terminating r c1) ->
+          terminating r c'.
+
+(* Theorem 3.6.1 *)
+
+Definition measure' (c': (ainstruction * alist * rstate) + bool) :=
+  match c' with
+  | inr b => 0
+  | inl c' => ailength (fst (fst (c'))) + allength (snd (fst (c')))
+  end.
+  
+Lemma measure_decrease
+  (c1 c2: (ainstruction * alist * rstate) + bool):
+  c1 ⟹__c c2 -> measure' c1 > measure' c2.
+Proof. intros. destruct H; simpl; omega. Qed.
+  
+Lemma compiling_terminates
+  (c': (ainstruction * alist * rstate) + bool):
+  terminating compile_step c'.
+Proof.
+  remember (measure' c') as n.
+  generalize dependent c'.
+  induction (lt_wf n) as [n _ IH].
+  intros.
+  constructor. intros.
+  assert(measure' c1 < measure' c').
+  { apply measure_decrease. apply H. }
+  apply (IH (measure' c1)).
+  - rewrite Heqn. apply H0.
+  - reflexivity.
+Qed.
+
+(*
+We will prove the big step semantics to be equivalent to the small 
+step semantics combined with the compile time checker
+*)
+
+(* Lemma 3.6.2 *)
+Lemma final_state_1 (d : com) (L : list) (s s' : state) :
+  (d,s) ⟹__b s' -> (c d,L,s) ⟹__s* (c Skip,L,s').
+Proof.
+  intros.
+  remember (d,s) as d'.
+  generalize dependent d.
+  generalize dependent s.
+  generalize dependent L.
+  induction H as [| | l s1 d |]; intros; injection Heqd'; intros; subst.
+  - apply star_refl.
+  - eapply star_step. apply SComp.
+    eapply star_trans. apply (IHbig_step1 (c c__2 :: L) s c__1).
+    reflexivity.
+    eapply star_step. apply SLoad.
+    apply (IHbig_step2 L s__2 c__2). reflexivity.
+  - eapply star_step. apply SLet.
+    eapply star_trans.
+    apply (IHbig_step (i (x, s x) :: L) (update s x ⊥) d).
+    reflexivity.
+    eapply star_step. apply SLoad.
+    eapply star_step. apply SSet.
+    apply star_refl.
+  - eapply star_step. apply SAss. apply star_refl.
+Qed.
+
+Lemma related_eq (s : state) (r r' : rstate) :
+  related_states s r -> related_states s r' -> r = r'.
+Proof.
+  intros.
+  apply functional_extensionality.
+  intros.
+  unfold related_states in H.
+  unfold related_states in H0.
+  destruct (H x) as [eq1 [eq2 eq3]].
+  destruct (H0 x) as [eq1' [eq2' eq3']]. 
+  destruct (r' x).
+  rewrite eq1 in eq1'. rewrite eq1'. reflexivity.
+  rewrite eq2 in eq2'. rewrite eq2'. reflexivity.
+  rewrite eq3 in eq3'. rewrite eq3'. reflexivity.
+Qed.
+
+Definition abstract_equivalent (s: state): rstate :=
+  (fun (x:string) =>
+     (match (s x) with
+     | ⊥ => ⊥__a
+     | -__u => -__a
+     | z => *__a
+      end)).
+
+Lemma equivalent_related (s:state):
+  related_states s (abstract_equivalent s).
+Proof.
+  unfold related_states; unfold abstract_equivalent.
+  repeat (try(split)); intros;
+    try(rewrite H; reflexivity);
+    try(destruct (s x); try (discriminate H); try(reflexivity));
+    try(destruct H; inversion H);
+    try(eexists; auto).
+Qed.
+
+Lemma update_related (s s': state) (r r': rstate) (x: string):
+  related_states s r ->
+  related_states s' r' ->
+  related_states (update s x (s' x)) (update r x (r' x)).
+Proof.
+  unfold related_states; unfold related_states; intros.
+  split.
+  - unfold update. destruct (string_dec x x0). apply H0. apply H.
+  - split.
+    unfold update. destruct (string_dec x x0). apply H0. apply H.
+     unfold update. destruct (string_dec x x0). apply H0. apply H.
+Qed.
+
+Lemma update_related_list
+  (L: List.list string) (s: state) (r: rstate):
+  related_states s r ->
+  related_states (update_list s L -__u) (update_list r L -__a).
+Proof.
+  generalize dependent s.
+  generalize dependent r. 
+  induction L; intros. 
+  - simpl. apply H.
+  - simpl.
+    assert(related_states (update s a -__u) (update r a -__a)).
+    { apply (update_related s (fun x => -__u) r (fun x => -__a) a).
+      apply H. unfold related_states. intros.
+      repeat(split); intros; 
+        try(discriminate H0); try(reflexivity).
+      destruct H0. discriminate H0. }
+    apply IHL. apply H0.
+Qed.
+
+Lemma unique_repr (s: state) (r r': rstate):
+  related_states s r -> related_states s r' -> r = r'. 
+Proof. 
+  unfold related_states. intros. 
+  apply functional_extensionality.
+  intros. destruct (r x) eqn: eq;
+  apply (H x) in eq; apply (H0 x) in eq; auto using eq.
+Qed.
+  
+Lemma update_abstract (s s': state) (r: rstate) (x: string):
+  related_states s r ->
+  update (abstract_equivalent s') x (r x) =
+  abstract_equivalent (update s' x (s x)).
+Proof.
+  intros.
+  assert(related_states (update s' x (s x))
+                        (update (abstract_equivalent s') x (r x))).
+  { apply update_related. apply equivalent_related. apply H. }
+  assert(related_states (update s' x (s x))
+                        ( abstract_equivalent (update s' x (s x)))).
+  { eapply equivalent_related.  }
+  eapply unique_repr. apply H0. apply H1. 
+Qed.
+
+Lemma expr_evaluation
+  (s: state) (e: expr) (y: string) (z: BinNums.Z):
+  In y (vars e) -> aval s e = val z -> (exists z', s y = val z'). 
+Proof.
+  intros.
+  generalize dependent z. 
+  induction e; intros; simpl in H; simpl in H.
+  - destruct H eqn: eq.
+    + eexists. rewrite e in H0. apply H0.
+    + exfalso. apply f.
+  - exfalso. apply H.
+  - apply in_app_or in H. destruct H.
+    + destruct (aval s e1) eqn: eq1; destruct (aval s e2) eqn: eq2;
+        try(simpl in H0) ; try (rewrite eq1 in H0) ;
+          try (rewrite eq2 in H0) ; try(discriminate H0).
+      apply (IHe1 H z0). reflexivity.
+    + destruct (aval s e1) eqn: eq1; destruct (aval s e2) eqn: eq2;
+        try(simpl in H0) ; try (rewrite eq1 in H0) ;
+          try (rewrite eq2 in H0) ; try(discriminate H0).
+      apply (IHe2 H z1). reflexivity. 
+ Qed.
+
+  
+Lemma final_state_2
+  (d : com) (L : alist) (s s': state) (r r' : rstate) :
+  (d,s) ⟹__b s' ->
+  related_states s r ->
+  related_states s' r' ->
+  inl (ac Skip, L, r') ⟹__c* inr true ->
+  inl (ac d, L, r) ⟹__c* inr true .
+Proof.
+  intros.
+  remember (d,s) as d'.
+  generalize dependent r.
+  generalize dependent s. 
+  generalize dependent d.
+  generalize dependent r'.
+  generalize dependent L.
+  induction H;
+    intros; injection Heqd'; intros; subst.
+  - rewrite <- (related_eq s0 r r') in H2.
+    apply H2. apply H0. apply H1. 
+  - eapply star_step. apply CSeq.
+    eapply (IHbig_step1 (ac c__2 :: L) (abstract_equivalent s__2)
+                        (equivalent_related s__2)).
+    eapply star_step. apply CSkipCons.
+    eapply IHbig_step2. apply H1. apply H2. eauto.
+    apply (equivalent_related s__2). eauto. apply H3.
+  - eapply star_step. apply CLet.
+    eapply IHbig_step. apply (equivalent_related s'). 
+    eapply star_step. apply CSkipCons.
+    eapply star_step. apply CBind.
+    rewrite (update_abstract s0 s' r x H0).
+    rewrite <- ((unique_repr (update s' x (s0 x)) r'
+           (abstract_equivalent (update s' x (s0 x)))) H1
+           (equivalent_related (update s' x (s0 x)))).
+    apply H2. eauto.
+    apply (update_related s0 (fun e => ⊥) r (fun e => ⊥__a)).
+    apply H0. unfold related_states. intros.
+    (* add as constant lemma *)
+    split. split. reflexivity. reflexivity.
+    split. split. discriminate. discriminate.
+    split. intros. destruct H3. discriminate H3.
+           intros. discriminate H3.
+  - eapply star_step. apply CAss_legal.
+    + simpl in H. apply H4. apply H.
+    + intros. destruct (aval s0 e) eqn: eq.
+      ++ contradiction H1. reflexivity.
+      ++ contradiction H0. reflexivity.
+      ++ assert(exists z', s0 y = val z').
+        { eapply expr_evaluation. apply H5. apply eq. }
+        apply H4. apply H6.
+    + intros. destruct (aval s0 e) eqn: eq.
+      ++ contradiction H1. reflexivity.
+      ++ contradiction H0. reflexivity.
+      ++ assert(related_states
+                 (update_list (update s0 x (val z)) (vars e) -__u)
+                 (update_list (update r x *__a) (vars e) -__a)).
+        { apply update_related_list.
+          apply (update_related s0 (fun n => val z) r (fun n => *__a)).
+          apply H4. unfold related_states. intros.
+          repeat(split); intros;
+            try(discriminate H5); try(eexists; eauto).
+        }
+        assert(r' = update_list (update r x *__a) (vars e) -__a).
+        { eapply unique_repr. apply H2. apply H5. }
+        rewrite <- H6. apply H3.     
+Qed.
+
+(* Todo: rewrite abstract_equivalent above with this definition *)
+Definition abstract_value (z: zext): abstract_zext :=
+  match z with
+  | ⊥ => ⊥__a
+  | -__u => -__a
+  | z => *__a
+  end.
+
+Fixpoint abstract_instruction (i': instruction): ainstruction :=
+  match i' with
+  | i (x, v) => ai (x, abstract_value v) 
+  | c v => ac v
+  end.
+
+Definition abstract_list (l: list): alist  :=
+  map abstract_instruction l.
+
+Lemma expr_eval (e: expr) (s: state) (r: rstate):
+  (forall y : string, In y (vars e) -> r y = *__a) ->
+  related_states s r ->
+  (exists z, aval s e = val z).
+Proof.
+  induction e; intros. 
+  - simpl. apply (H0 v). apply (H v). simpl. auto.
+  - simpl. eexists. auto.
+  - assert(exists z : BinNums.Z, aval s e1 = val z).
+    { eapply IHe1. intros. apply H. simpl. 
+      apply in_or_app. left. apply H1. apply H0. }
+    assert(exists z : BinNums.Z, aval s e2 = val z).
+    { eapply IHe2. intros. apply H. simpl. 
+      apply in_or_app. right. apply H2. apply H0. }
+    destruct H1. destruct H2. eexists. simpl.
+    rewrite H1. rewrite H2. auto.
+Qed.
+
+Lemma related_abstract_values (s: state) (r: rstate) (x: string):
+  related_states s r ->
+  r x = abstract_value (s x).
+Proof.
+  intros. unfold related_states in H.
+  destruct (s x) eqn: eq; apply (H x);
+    try(apply eq) ; try(eexists; apply eq).  
+Qed.
+  
+(* Lemma 3.6.3 *)
+Lemma compile_one_step
+  (d d': instruction) (l l': list) (s s': state) (r: rstate):
+  ((d, l, s) ⟹__s (d', l', s')) ->
+  related_states s r ->
+  inl (abstract_instruction d, abstract_list l, r) ⟹__c* inr true ->
+  (exists (r': rstate),
+      related_states s' r' /\
+      (inl (abstract_instruction d, abstract_list l, r) ⟹__c
+      inl (abstract_instruction d', abstract_list l', r'))).
+Proof.
+  intros.
+  inversion H; subst; simpl. 
+  - inversion H1. subst. inversion H2. subst.
+    eexists. split. apply H0. apply H2.
+  - inversion H1. subst. inversion H2. subst.
+    eexists. split. apply H0. apply H2.
+  - inversion H1. subst. inversion H2. subst.
+    eexists. split.
+    + apply update_related_list.
+      apply (update_related s (fun n => aval s e) r (fun n => *__a)).
+      apply H0.
+      assert(exists z, aval s e = val z).
+      { eapply expr_eval. apply H10. apply H0. }
+      destruct H4. rewrite H4.
+      unfold related_states. intros.
+      repeat(split); intros; try(discriminate H5).
+      eexists. auto.
+    + apply H2.
+    + subst. inversion H3. inversion H4.
+  - inversion H1. subst. inversion H2. subst.
+    eexists. split.
+    + apply (update_related s (fun n => ⊥) r (fun n => ⊥__a)).
+      apply H0. unfold related_states. intros.
+      repeat(split); intros; try(discriminate H4);
+        try(destruct H4; discriminate H4; auto).
+    + assert(r x = abstract_value (s x)). 
+      { apply related_abstract_values. apply H0. }
+      rewrite <- H4. apply H2.
+  - inversion H1. subst. inversion H2. subst.
+    simpl in H2. eexists. split.
+    apply (update_related s (fun n => v) r (fun n => abstract_value v)).
+    apply H0. unfold related_states. intros.
+    repeat(split); intros; destruct v;
+      try(discriminate H4); try(reflexivity);
+        try(destruct H4; discriminate H4).
+    eexists. eauto. apply H2.
+Qed.
+
+Lemma compile_deterministic_one_step
+  (conf conf1 conf2: ainstruction * alist * rstate + bool):
+  (conf ⟹__c conf1) -> (conf ⟹__c conf2) -> conf1 = conf2.
+Proof.
+  intros.
+  inversion H; subst; inversion H0; subst; try(reflexivity).
+  - exfalso. destruct H8.
+    ++ contradiction.
+    ++ destruct H3 as [y [H3 H3']]. apply H3'.
+      apply (H2 y). apply H3.
+  -  exfalso. destruct H1.
+    ++ contradiction.
+    ++ destruct H1 as [y [H1 H1']]. apply H1'.
+      apply (H8 y). apply H1.
+Qed.
+
+Lemma compile_deterministic_truth
+  (conf conf': ainstruction * alist * rstate + bool):
+  (conf ⟹__c* conf') -> (conf ⟹__c* inr true) -> conf' ⟹__c* inr true.
+Proof.
+  intros.
+  induction H.
+  - apply H0.
+  - apply IHstar.
+    inversion H0; subst.
+    + inversion H.
+    + assert(y = y0).
+      { eapply compile_deterministic_one_step. apply H. apply H2. }
+      rewrite <- H4 in H3. apply H3.
+Qed.
+
+(* Lemma 3.6.4 *)
+Lemma compile_steps
+  (d d': instruction) (l l': list) (s s': state) (r: rstate):
+  ((d, l, s) ⟹__s* (d', l', s')) ->
+  related_states s r ->
+  inl (abstract_instruction d, abstract_list l, r) ⟹__c* inr true ->
+  (exists (r': rstate),
+      related_states s' r' /\
+      (inl (abstract_instruction d, abstract_list l, r) ⟹__c*
+      inl (abstract_instruction d', abstract_list l', r'))).
+Proof.
+  intros H.
+  remember (d, l, s) as conf1.
+  remember (d',l', s') as conf2.
+  generalize dependent d.
+  generalize dependent d'.
+  generalize dependent l.
+  generalize dependent l'.
+  generalize dependent s.
+  generalize dependent s'.
+  generalize dependent r. 
+  dependent induction H.
+  - intros. rewrite Heqconf1 in Heqconf2. injection Heqconf2.
+    intros. subst. exists r. split. apply H. apply star_refl.
+  - intros. subst. destruct y as [[d1 l1] s1].
+    assert(exists r' : rstate, related_states s1 r' /\
+      (inl (abstract_instruction d, abstract_list l, r)
+    ⟹__c inl (abstract_instruction d1, abstract_list l1,
+            r'))).
+    { eapply compile_one_step. apply H. apply H1. apply H2. }
+    destruct H3 as [r1 [H3 H3']].
+    assert( exists r' : rstate,
+         related_states s' r' /\
+         inl (abstract_instruction d1, abstract_list l1, r1)
+       ⟹__c* inl (abstract_instruction d', abstract_list l', r')).
+    { eapply IHstar. reflexivity. eauto. apply H3.
+      inversion H2. 
+      + subst.
+        assert(y = inl (abstract_instruction d1,
+                        abstract_list l1, r1)).
+        { eapply compile_deterministic_one_step.
+          apply H4. apply H3'. }
+        rewrite H6 in H5. apply H5.
+    }
+    destruct H4 as [r2 [H4 H4']].
+    eexists. split. apply H4. eapply star_step.
+    apply H3'. apply H4'.
+Qed.
+
+(* Lemma 3.6.5 *)
+Lemma small_to_big
+  (d: com) (l: list) (s s': state) (r: rstate):
+  ((c d, l, s) ⟹__s* (c Skip, l, s')) ->
+  related_states s r ->
+  inl (abstract_instruction (c d), abstract_list l, r)
+      ⟹__c* inr true ->
+  (d, s) ⟹__b s'.
+Proof.
+  generalize dependent l.
+  generalize dependent s'.
+  generalize dependent s.
+  generalize dependent r. 
+  induction d; intros. 
+  - assert(s = s'). { eapply between_skips. apply H. }
+    rewrite H2. apply BSkip.
+  - destruct (comp_to_skip d1 d2 l s s' H) as [s2 [H4 [H4' h4']]].
+    eapply BSeq. eapply IHd1. 
+    inversion H. subst. inversion H2. subst.    
+    eapply H4. eapply H0.
+    inversion H1. subst. inversion H2. subst.
+    apply H3.
+    eapply IHd2. apply h4'.
+    apply (equivalent_related s2).
+    inversion H1. subst. inversion H2. subst.
+    eapply compile_deterministic_truth.
+    destruct (compile_steps (c d1) (c Skip) (c d2 :: l) (c d2 :: l)
+                            s s2 r H4 H0 H3) as [r5 [H5 H5']].
+    assert(r5 = abstract_equivalent s2).
+    { eapply unique_repr. apply H5. apply equivalent_related. }
+    rewrite H6 in H5'.
+    assert(inl (abstract_instruction (c d1),
+                abstract_list (c d2 :: l), r) ⟹__c* inl
+          (abstract_instruction (c d2), abstract_list l,
+          abstract_equivalent s2)). 
+    { apply plus_star. eapply plus_right. apply H5'.
+      apply CSkipCons. }
+    apply H7. apply H3.
+  - inversion H. subst. inversion H2. subst.
+    inversion H1. subst. inversion H4. subst.
+    destruct (let_to_skip d l s s' t v H) as [s2 [eq1 [eq2 eq3]]].
+    inversion eq3. subst. inversion H6. subst.
+    assert(update s2 v (s v) = s').
+    { eapply between_skips. apply H7. }
+    rewrite <- H8.
+    apply BLet. eapply IHd.
+    inversion eq1. subst. inversion H9. subst.
+    apply H10.
+    apply (update_related s (fun n => ⊥) r (fun n => ⊥__a)).
+    apply H0. unfold related_states.
+    repeat(split); intros; try(discriminate H9); try(reflexivity);
+      try(destruct H9; discriminate H9).
+    assert(r v = abstract_value (s v)).
+    { apply related_abstract_values. apply H0. }
+    simpl. rewrite <- H9. apply H5. 
+  - inversion H. subst. inversion H2. subst.
+    inversion H1. subst. inversion H4. subst.
+    assert(update_list (update s v (aval s e)) (vars e) -__u = s').
+    { eapply between_skips. apply H3. }
+    rewrite <- H6. apply BAssign. 
+    + auto.
+    + simpl.
+      assert(r v = abstract_value (s v)). 
+      { apply (related_abstract_values s r v). apply H0. }
+      rewrite H11 in H7.
+      destruct (s v); simpl in H7;
+        try(discriminate H7); try(reflexivity).
+    + destruct (expr_eval e s r H12 H0).
+      rewrite H7. unfold not. intros. discriminate H8.
+    + destruct (expr_eval e s r H12 H0).
+      rewrite H7. unfold not. intros. discriminate H8.
+    + subst. inversion H5. subst. inversion H6.
+Qed.
+
+(* Lemma 3.6.6 *)
+Lemma small_big
+  (d: com) (s s': state) (r: rstate):
+  (d, s) ⟹__b s' <->
+  (exists l, ((c d, l, s) ⟹__s* (c Skip, l, s')) /\
+  related_states s (abstract_equivalent s) /\
+  inl (abstract_instruction (c d), abstract_list l,
+       (abstract_equivalent s))
+      ⟹__c* inr true).
+Proof.
+  split; intros.
+  - exists nil. split.
+    + apply final_state_1. apply H.
+    + split. apply (equivalent_related s).
+      eapply final_state_2. apply H. apply (equivalent_related s).
+      apply (equivalent_related s').
+      eapply star_step. apply CSkipNil. apply star_refl.
+  - destruct H as [l [eq1 [eq2 eq3]]].
+    eapply small_to_big. apply eq1. apply (equivalent_related s).
+    apply eq3.
+Qed.
+
+(*
+Preservation
+
+If the compile time checker says a program is okay and 
+you take a step in the semantics, the checker will say 
+it is still okay.
+*)
+
+(* Lemma 3.6.7 *)
+Lemma preservation
+  (d d': instruction) (s s': state) (r: rstate) (l l': list):
+  inl (abstract_instruction d, abstract_list l, r) ⟹__c* inr true ->
+  ((d, l, s) ⟹__s (d', l', s')) ->
+  related_states s r ->
+  (exists r', related_states s' r' /\
+         inl (abstract_instruction d', abstract_list l', r') ⟹__c*
+         inr true). 
+Proof.
+  intros.
+  inversion H0; subst.
+  - inversion H; subst. inversion H2; subst.
+    eexists. split. apply H1. apply H3. 
+  - inversion H; subst. inversion H2; subst.
+    eexists. split. apply H1. apply H3.
+  - inversion H; subst. inversion H2; subst.
+    eexists. split.
+    + apply update_related_list.
+      assert(exists z, aval s e = val z).
+      { eapply expr_eval. apply H10. apply H1. }
+      apply (update_related s (fun n => aval s e) r (fun n => *__a)).
+      apply H1. destruct H4 as [z H4]. rewrite H4. 
+      repeat(split); intros; try(discriminate H5).
+      eexists. eauto.
+    + apply H3.
+    + inversion H3. inversion H4.
+  - inversion H; subst. inversion H2; subst.
+    eexists. split. 
+    + apply (update_related s (fun n => ⊥) r (fun n => ⊥__a)).
+      apply H1. 
+      repeat(split); intros; try(destruct H4; discriminate H4);
+        try(discriminate H4).
+    + simpl.
+      assert(r x = abstract_value (s x)).
+      { apply related_abstract_values. apply H1. }
+      rewrite <- H4. apply H3. 
+  - inversion H; subst. inversion H2; subst.
+    eexists. split.
+    + apply (update_related s (fun n => v) r
+            (fun n => abstract_value v)).
+      apply H1.
+      repeat(split); intros; destruct v;
+        try (discriminate H4); try(eauto);
+          try(destruct H4; discriminate H4).
+    + apply H3. 
+Qed.
+
+(*
+Progress
+
+If the program passes through the compile time checker, 
+we can always do a step in the semantics.
+ *)
+
+Lemma invert_skip (d: instruction):
+  ac Skip = abstract_instruction d -> d = c Skip. 
+Proof.
+  destruct d; intros.
+  - destruct p. simpl in H. discriminate H.
+  - simpl in H. injection H. intros. rewrite H0. reflexivity.
+Qed.
+
+Lemma invert_nil (l: list):
+  nil = abstract_list l -> l = nil. 
+Proof.
+  destruct l; intros.
+  - reflexivity.
+  - simpl in H. discriminate H.
+Qed.
+
+Lemma invert_cons (l: list) (p: ainstruction) (l0: alist):
+  p :: l0 = abstract_list l ->
+  (exists p' l0', l = p' :: l0'). 
+Proof.
+  intros.
+  destruct l as [|i' l']. 
+  - simpl in H. discriminate H.
+  - simpl in H. exists i'. exists l'. reflexivity.
+Qed.
+
+(* Todo: remove skip_nil *)
+Lemma invert_command (c': com) (d: instruction):
+  ac c' = abstract_instruction d -> d = c c'. 
+Proof.
+  destruct d; intros.
+  - simpl in H. destruct p. discriminate H. 
+  - destruct c'; intros; simpl in H;
+      try(injection H; intros; rewrite H0; reflexivity).
+Qed.
+
+Lemma invert_binding
+  (x: vname) (av: abstract_zext) (d: instruction):
+  ai (x, av) = abstract_instruction d ->
+  (exists cv, d = i (x, cv)). 
+Proof.
+  destruct d; intros.
+  - destruct p. simpl in H. injection H. intros.
+    exists z. rewrite H1. reflexivity.
+  - simpl in H. discriminate H.
+Qed.
+
+(* Lemma 3.6.9 *)
+Lemma progresss
+  (d: instruction) (r: rstate) (l: list):
+  inl (abstract_instruction d, abstract_list l, r) ⟹__c* inr true ->
+  (d = c Skip /\ l = nil) \/
+  (forall s, related_states s r ->
+        (exists d' l' s', (d, l, s) ⟹__s (d', l', s'))).
+Proof.
+  intros.
+  inversion H; subst. inversion H0; subst.
+  - left. split.
+    apply invert_skip. apply H3.
+    apply invert_nil. apply H4.
+  - right. intros.
+    apply invert_cons in H4.
+    destruct H4 as [p' [l0' H4]].
+    exists p'. exists l0'. exists s.
+    apply invert_skip in H3. rewrite H3. rewrite H4.
+    apply SLoad.
+  - right. intros. 
+    apply invert_command in H3. rewrite H3.
+    repeat(eexists). apply SComp.
+  - right. intros.
+    apply invert_command in H2. rewrite H2.
+    repeat(eexists). apply SAss.
+  - right. intros.
+    apply invert_command in H2. rewrite H2.
+    repeat(eexists). apply SAss.
+  - right. intros.
+    apply invert_command in H3. rewrite H3.
+    repeat(eexists). apply SLet.
+  - right. intros.
+    apply invert_binding in H3. destruct H3. rewrite H3.
+    repeat(eexists). apply SSet.
+Qed.
