capabilities/small_step.v
@@ -1,0 +1,897 @@
+Set Warnings "-notation-overridden,-parsing".
+(*
+Author: Rodrigo Raya
+
+Following "The Semantics of Ownership and Borrowing in the Rust Programming Language" by Nienke Wessel.
+*)
+
+From Coq Require Import Bool.Bool.
+From Coq Require Import Init.Nat.
+From Coq Require Import Arith.Arith.
+From Coq Require Import ZArith.Int.
+From Coq Require Import Arith.EqNat.
+From Coq Require Import omega.Omega.
+From Coq Require Import Lists.List.
+From Coq Require Import Strings.String.
+From Coq Require Import Logic.FunctionalExtensionality.
+(* for specific induction *)
+Require Import Coq.Program.Equality.
+Require Import Capabilities.big_step.
+
+Import ListNotations.
+Open Scope string_scope.
+Open Scope list_scope.
+
+(* Small-step semantics *)
+
+Inductive instruction :=
+| prog_instr : vname * zext -> instruction
+| command : com -> instruction.
+
+Notation "'c' com" := (command com) (at level 20) : move_scope.
+Notation "'i' p_instr" := (prog_instr p_instr) (at level 20) : move_scope.
+
+Definition list := list instruction.
+
+Reserved Notation "e '⟹__s' b" (at level 120, left associativity).
+
+Inductive small_step : instruction * list * state ->
+                        instruction * list * state -> Prop :=
+| SLoad (s: state) (I: instruction) (L: list) :
+    (c Skip, I :: L, s) ⟹__s (I,L,s)
+| SComp (s : state) (c__1 c__2: com) (L : list) :
+    (c  (c__1;;c__2),L,s) ⟹__s  (c c__1, c c__2 :: L,s)
+| SAss (s : state) (e : expr) (x: string) (L : list) :
+    (c (x ;= e),L,s) ⟹__s
+     (c Skip,L,update_list (update s x (aval s e)) (vars e) -__u)                 
+| SLet (s : state) (c' : com) (x : vname) (t : type) (L:list) :
+    (c (LET x , t IN c'), L, s) ⟹__s
+     (c c', i (x, (s x)) :: L, update s x ⊥)
+| SSet (s : state) (x : string) (v : zext) (L : list) :
+    (i (x,v),L,s) ⟹__s (c Skip,L, update s x v)                                    
+where "e '⟹__s' b" := (small_step e b) : move_scope.
+
+Lemma deterministic_one_step
+  (conf conf1 conf2: instruction * list * state) :
+  (conf ⟹__s conf1) ->
+  (conf ⟹__s conf2) ->
+  conf1 = conf2.
+Proof. intros. induction H; inversion H0; subst; reflexivity. Qed.
+
+Inductive star {A : Type} (r : A -> A -> Prop) : A -> A -> Prop :=
+| star_refl x : star r x x
+| star_step x y z : r x y -> star r y z -> star r x z.
+
+Notation "x '⟹__s*' y" := (star small_step x y) (at level 20) : move_scope.
+
+Lemma star_trans {A} (r : A -> A -> Prop) :
+  forall x y z, star r x y -> star r y z -> star r x z.
+Proof.
+  intros x y z H1 H2.
+  generalize dependent z.
+  induction H1; intros.
+  - apply H2.
+  - apply ((star_step r x y z0) H (IHstar z0 H2)).
+Qed.
+
+Lemma star_step' {A} (r : A -> A -> Prop) :
+  forall x y, r x y -> star r x y.
+Proof.
+  intros x y H.
+  apply (star_step r x y y).
+  + apply H.
+  + apply star_refl.
+Qed.
+
+Inductive splus {A : Type} (r : A -> A -> Prop) : A -> A -> Prop :=
+| plus_step x y : r x y -> splus r x y
+| plus_steps x y z : r x y -> star r y z -> splus r x z.
+
+Notation "x '⟹__s+' y" := (splus small_step x y) (at level 30) : move_scope.
+
+Lemma plus_star {A} (r : A -> A -> Prop) :
+  forall x y, splus r x y -> star r x y.
+Proof.
+  intros x y H.
+  induction H.
+  - apply star_step'. apply H.
+  - eapply star_step. apply H. apply H0.
+Qed.
+
+Lemma plus_right {A} (r : A -> A -> Prop) :
+  forall x y z, star r x y -> r y z -> splus r x z.
+Proof.
+  intros x y z H1 H2.
+  induction H1.
+  - apply plus_step. apply H2.
+  - eapply plus_steps. apply H.
+    eapply star_trans. apply H1.
+    eapply star_step. apply H2. apply star_refl.
+Qed.
+  
+(* Traces *)
+
+Definition trace
+           (f: nat -> (instruction * list * state)) (m: nat)
+           (c1 c2: instruction * list * state)  :=      
+    (f 0 = c1) /\ (f m = c2) /\ 
+    (forall (idx:nat), (0 <= idx /\ idx < m) -> f idx ⟹__s f (S idx)).
+
+Lemma small_trace (i1 i2 : instruction) (L1 L2 : list) (s1 s2 : state):
+  (i1, L1, s1) ⟹__s* (i2, L2,s2) ->
+  (exists (f : nat -> (instruction * list * state)) (m : nat),
+      trace f m (i1,L1,s1) (i2,L2,s2)).
+Proof.
+  intros. unfold trace.
+  dependent induction H generalizing i1 i2 L1 L2 s1 s2.
+  - exists (fun n => (i2,L2,s2)). exists 0.
+    split. reflexivity. split. reflexivity. 
+    intros. omega.
+  - destruct y as [p s']; destruct p as [i' l'].
+    destruct (IHstar i' i2 l' L2 s' s2) as [g]; try(reflexivity).
+    destruct H1 as [m]. 
+    exists (fun n => match n with
+                   | 0 => (i1, L1,s1)
+                   | S n' => g n' end). exists (S m).
+    destruct H1 as [eq1 [eq2 eq3]].
+    split; try(reflexivity). split. 
+    + destruct (S m) eqn: m_plus_1.
+      ++ omega. 
+      ++ apply eq2.
+    + intros.
+      destruct idx.
+      ++ simpl. rewrite eq1. apply H. 
+      ++ simpl.
+        assert(0 <= idx < m). { omega. }
+        apply (eq3 idx H2).
+Qed.
+
+Lemma trace_connected
+      (f: nat -> (instruction * list * state)) (m:nat)
+      (c1 c2: instruction * list * state) :
+  trace f m c1 c2 -> (forall j, 0 <= j <= m -> (f j ⟹__s* c2 /\ c1 ⟹__s* f j)).
+Proof.
+  intros. unfold trace in H. destruct H as [H1 [H2 H3]]. split.
+  - generalize dependent c2. 
+    induction m; intros. 
+    + assert(j = 0). { omega. } subst. apply star_refl. 
+    + destruct (Nat.eqb_spec j (S m)).
+      ++ subst. apply star_refl.
+      ++ assert(eq1: 0 <= j <= m). { omega. }
+        assert(eq2: forall idx : nat, 0 <= idx < m -> f idx ⟹__s f (S idx)).
+        { intros. apply H3. omega. }
+        assert(f j ⟹__s* f m).
+        { apply ((IHm eq2 eq1) (f m)). reflexivity. }
+        assert(f m ⟹__s* f (S m)).
+        { apply star_step'. apply (H3 m). omega. }
+        subst. eapply star_trans. apply H. apply H4.
+  - generalize dependent c2. 
+    induction j; intros. 
+    + subst. apply star_refl.
+    + assert(c1 ⟹__s* f j). { eapply IHj. omega. apply H2. }
+      assert(f j ⟹__s* f (S j)). { apply star_step'. apply H3. omega. }
+      eapply star_trans. apply H. apply H4.
+Qed.
+
+Corollary small_trace'
+  (i1 i2 : instruction) (L1 L2 : list) (s1 s2 : state)
+  (f : nat -> (instruction * list * state)) (m : nat):
+  trace f m (i1,L1,s1) (i2,L2,s2) ->
+  (i1, L1, s1) ⟹__s* (i2, L2,s2).
+Proof.
+  intros. 
+  destruct (trace_connected f m (i1,L1,s1) (i2,L2,s2) H 0).
+  - omega.
+  - unfold trace in H. destruct H as [eq1 [eq2 eq3]].
+    rewrite eq1 in H0. apply H0.
+Qed.
+
+Lemma move_trace_right
+  (f: nat -> (instruction * list * state)) (m:nat)
+   (c1 c2 : instruction * list * state):    
+   trace f (S m) c1 c2 ->
+   trace (fun n  => f (S n)) (m) (f 1) c2.
+Proof.
+  intros. unfold trace. unfold trace in H.
+  destruct H as [H1 [H2 H3]].
+  split. reflexivity. split.
+  - apply H2.
+  - intros. apply (H3 (S idx)). omega. 
+Qed.
+
+Lemma compute_trace_step
+  (f: nat -> (instruction * list * state)) (m:nat)
+  (conf conf1 conf2: instruction * list * state) :
+  trace f (S m) conf1 conf2 ->
+  (conf1 ⟹__s conf) ->
+  trace (fun n => f (S n)) m conf conf2.
+Proof.
+  intros.
+  destruct conf1 as [[c1 l1] s1].
+  destruct conf2 as [[c2 l2] s2].
+  assert((c1,l1,s1) ⟹__s f 1).
+  { destruct H as [eq1 [eq2 eq3]]. rewrite <- eq1. apply eq3. omega. }
+  assert(f 1 = conf).
+  { eapply deterministic_one_step. apply H1. apply H0. }
+  rewrite <- H2. 
+  eapply move_trace_right. apply H.
+Qed.
+
+(* Helper measure that decreases on traces *)
+
+Fixpoint atomic_commands (c': com) :=
+  match c' with
+  | Skip => 1
+  | c1 ;; c2 => atomic_commands c1 + atomic_commands c2
+  | LET x , t IN b  => 1 + atomic_commands b
+  | x ;= e => 1
+  end.
+
+Lemma atomic_positive (c': com) : atomic_commands c' > 0.
+Proof. induction c'; simpl; omega. Qed.
+
+Fixpoint command_number (l: list) :=
+  match l with
+  | [] => 0
+  | c c' :: l => atomic_commands c' + command_number l
+  | i p :: l => 1 + command_number l
+  end.
+
+Lemma commands_gr_1 (i': instruction): command_number ([i']) > 0.
+Proof.
+  simpl. destruct i' as [| c']. omega.
+  assert(atomic_commands c' > 0). { apply atomic_positive. } omega. 
+Qed.
+
+Definition measure (instr: instruction) (L: list) :=
+  command_number [instr] + command_number L.       
+   
+Lemma step_decrease
+  (instr1 instr2 : instruction)
+   (L1 L2 : list) (s1 s2 : state) :
+  ((instr1, L1, s1) ⟹__s (instr2, L2, s2)) ->
+  (measure instr2 L2 <= measure instr1 L1).
+Proof.
+  intros. unfold measure.
+  destruct instr1.
+  - inversion H. subst. auto. 
+  - inversion H; subst; try(auto).
+    + simpl. destruct instr2.
+      ++ auto.
+      ++ omega.
+    + simpl. omega.
+    + simpl. omega.
+Qed.
+
+Lemma chain_decrease
+   (instr1 instr2 : instruction)  
+   (L1 L2 : list) (s1 s2 : state) :
+  ((instr1, L1, s1) ⟹__s* (instr2, L2, s2)) ->
+  (measure instr2 L2 <= measure instr1 L1).
+Proof.
+  intros H. unfold measure. 
+  dependent induction H generalizing instr1 L1 s1 instr2 L2 s2.
+  + auto.
+  + intros. subst.
+    destruct y as [p3 s3]. destruct p3 as [instr3 L3].
+    assert (H2: command_number [instr3] + command_number L3 <=
+            command_number [instr1] + command_number L1).
+    { eapply step_decrease. apply H. }
+    assert (H3: command_number [instr2] + command_number L2 <=
+                command_number [instr3] + command_number L3).
+    { eapply IHstar. auto. auto. }
+    omega.
+Qed.
+
+Lemma skip_decrease
+ (instr2 : instruction) (L1 L2 : list) (s1 s2 : state) :
+  ((c Skip, L1, s1) ⟹__s+ (instr2, L2, s2)) -> 
+  (measure instr2 L2 < measure (c Skip) L1).
+Proof.
+ intros H. unfold measure.
+ remember (c Skip, L1, s1) as conf1.
+ remember (instr2, L2, s2) as conf2. 
+ destruct H as [H1 | H2 ] eqn: H3. 
+ - intros. subst. inversion s. subst. simpl.
+   destruct instr2. omega. omega.
+  - intros. subst. inversion s. subst.
+    assert(command_number [I] + command_number L <
+           command_number [c Skip] + command_number (I::L)).
+    { simpl. destruct I.
+      + auto.
+      + omega. }
+    assert(command_number [instr2] + command_number L2 <=
+           command_number [I] + command_number L).
+    { eapply chain_decrease. apply s0.  }
+    omega.
+Qed.
+
+Corollary pop_changes_stacks_identity
+  (l l': list) (s s': state) (i': instruction):
+  (c Skip,l,s) ⟹__s+ (i',l',s') -> l <> l'.
+Proof.
+  intros.
+  assert(measure i' l' < measure (c Skip) l).
+  { eapply skip_decrease. apply H. }
+  assert(command_number [i'] > 0). { apply commands_gr_1. }
+  assert(command_number l' < command_number l).
+  { unfold measure in H0. simpl in H0. simpl in H1. omega. } 
+  intros contra.
+  assert(command_number l' = command_number l).
+  { rewrite contra. reflexivity. }
+  omega.
+Qed.
+
+
+Lemma move_plus (c1 c2 c1' c2' : instruction * list * state ) :
+  (c1 ⟹__s+ c2) ->
+   (c1 ⟹__s c1') ->
+   (c2 ⟹__s c2') ->
+   (c1' ⟹__s+ c2').
+Proof.
+  intros. 
+  assert(c1' ⟹__s* c2).
+  { inversion H; subst.
+    + rewrite (deterministic_one_step c1 c1' c2 H0 H2).
+      apply star_refl.
+    + rewrite (deterministic_one_step c1 c1' y H0 H2).
+      apply H3. } 
+  eapply plus_right. apply H2. apply H1.
+Qed.
+
+Lemma no_loops ( c1 c2 : instruction * list * state ) :
+  ((c1 ⟹__s+ c2) -> c1 = c2 -> False).
+Proof.
+  intros H.
+  destruct c1 as [[i1 l1] s1].
+  induction i1 as [p | c']; subst.
+  + intros. subst. destruct p as [x v]. 
+    assert((c Skip, l1, update s1 x v) ⟹__s+
+           (c Skip, l1, update s1 x v)).
+      { eapply move_plus. apply H. apply SSet. apply SSet. }
+    assert(l1 <> l1).
+      { eapply pop_changes_stacks_identity. apply H0. }
+      apply H1. reflexivity.
+  + generalize dependent c2.
+    generalize dependent l1.
+    generalize dependent s1.
+    induction c'; intros; subst.
+    ++ assert(l1 <> l1).
+      { eapply pop_changes_stacks_identity. apply H. }
+      apply H0. reflexivity.
+    ++ assert((c c'1, c c'2 :: l1, s1) ⟹__s+ (c c'1, c c'2 :: l1, s1)).
+      { eapply move_plus. apply H. apply SComp. apply SComp. }
+      eapply IHc'1. apply H0. reflexivity.
+    ++ assert((c c', i (v, s1 v) :: l1, update s1 v ⊥) ⟹__s+
+             (c c', i (v, s1 v) :: l1, update s1 v ⊥)).
+      { eapply move_plus. apply H. apply SLet. apply SLet. }
+      eapply IHc'. apply H0. reflexivity.     
+    ++ assert((c Skip, l1,
+             update_list (update s1 v (aval s1 e)) (vars e) -__u) ⟹__s+
+             (c Skip, l1,
+             update_list (update s1 v (aval s1 e)) (vars e) -__u)).
+      { eapply move_plus. apply H. apply SAss. apply SAss. }
+      assert(l1 <> l1).
+      { eapply pop_changes_stacks_identity. apply H0. }
+      apply H1. reflexivity.
+Qed.
+
+(* Stack *)
+
+Lemma pop_skip (i1 i2 i': instruction) (l : list) (s1 s2: state) :
+  ((i1,i'::l,s1) ⟹__s (i2,l,s2)) ->
+  i1 = c Skip  /\ s1 = s2.
+Proof.
+  intros. inversion H.
+  - split; reflexivity.
+  - assert(List.length (c c__2 :: i' :: l) = List.length l).
+    { rewrite H5. reflexivity. }
+    simpl in H0. omega.
+  - assert(List.length (i' :: l) = List.length l).
+    { rewrite H5. reflexivity. }
+    simpl in H0. omega.
+  - assert(List.length (i (x, s1 x) :: i' :: l) = List.length l).
+    { rewrite H5. reflexivity. }
+    simpl in H0. omega.
+  - assert(List.length (i' :: l) = List.length l).
+    { rewrite H5. reflexivity. }
+    simpl in H0. omega.
+Qed.
+
+(*
+Lemma push_let_comp
+   (i1 i2 i': instruction) (l : list) (s1 s2: state) :
+  ((i1,l,s1) ⟹__s (i2,i'::l,s2)) ->
+  (exists c1 c2, i1 = c (c1 ;; c2)  /\ s1 = s2) \/
+  (exists x t c', i1 = c (LET x , t IN c') /\ s2 = update s1 x (s1 x)).
+Proof.
+  intros.
+  inversion H; subst. 
+  - 
+Admitted.
+*)
+
+Lemma stack_changes (i1 i2: instruction) (l1 l2 : list) (s1 s2: state) :
+  ((i1,l1,s1) ⟹__s (i2,l2,s2)) ->
+  (l1 = l2 \/ (exists push, l2 = push :: l1) \/ (exists pop, l1 = pop :: l2)).
+Proof.
+  intros. 
+  inversion H; subst. 
+  - right. right. eauto.
+  - right. left. eauto.
+  - left. eauto. 
+  - right. left. eauto.  
+  - left. eauto. 
+Qed.
+
+Lemma stack_size_changes
+  (i1 i2: instruction) (l1 l2 : list) (s1 s2: state) :
+  ((i1,l1,s1) ⟹__s (i2,l2,s2)) ->
+  List.length l1 = List.length l2 \/
+  List.length l1 = List.length l2 + 1 \/
+  List.length l1 + 1 = List.length l2.
+Proof.
+  intros. 
+  destruct (stack_changes i1 i2 l1 l2 s1 s2 H)
+    as [eq1 | [eq2 | eq3]].
+  - left. rewrite eq1. reflexivity.
+  - right. right. destruct eq2. rewrite H0. simpl. omega.
+  - right. left. destruct eq3. rewrite H0. simpl. omega.
+Qed.
+
+Lemma stack_size_changes_explicit
+  (conf1 conf2: instruction * list * state) :
+  ((conf1 ⟹__s conf2) ->
+  (List.length (snd (fst (conf1))) <>
+  List.length (snd (fst (conf2)))) ->
+  (List.length (snd (fst (conf1))) <>
+  List.length (snd (fst (conf2))) + 1) ->
+  (List.length (snd (fst (conf1))) + 1 <>
+  List.length (snd (fst (conf2)))) ->
+  False).
+Proof.
+  intros.
+  destruct conf1 as [[i1' l1] s1].
+  destruct conf2 as [[i2' l2] s2].
+  simpl in H0. simpl in H1. simpl in H2.
+  destruct (stack_size_changes i1' i2' l1 l2 s1 s2 H)
+    as [eq1 | [eq2 | eq3]]; omega. 
+Qed.
+    
+Definition trace_not_below
+  (f: nat -> (instruction * list * state)) (m:nat) (l2: list) :=
+  (forall j, 0 <= j < m -> (exists l', snd(fst (f j)) = l' ++ l2)).
+
+Lemma trace_below_right
+  (f: nat -> (instruction * list * state)) (m:nat) (l:list):
+  ((exists l', snd (fst (f 0)) = l' ++ l) /\
+   trace_not_below (fun n : nat => f (S n)) m l) ->
+  trace_not_below f (S m) l.
+Proof.
+  intros. destruct H as [H1 H2].
+  unfold trace_not_below. unfold trace_not_below in H2.
+  intros. destruct j.
+  - apply H1.
+  - apply H2. omega.
+Qed.
+
+(* push lemma *)
+Lemma not_below
+  (f: nat -> (instruction * list * state)) (m:nat)
+  (c1 c2: instruction) (s1 s2: state) (l1 l2: list) :
+  trace f m (c1,l1++l2,s1) (c2,l2,s2) ->
+  trace_not_below f m l2.
+Proof.
+  unfold trace_not_below. intros. 
+  remember H as tr.
+  unfold trace. destruct H as [eq1 [eq2 eq3]].
+  induction j.
+  + exists l1. rewrite eq1. reflexivity.
+  + destruct IHj as [lj]; try(omega).
+    assert(f j ⟹__s f (S j)). { apply eq3. omega. }
+    assert(f j ⟹__s+ (c2,l2,s2)). {
+      assert(f (S j) ⟹__s* (c2,l2,s2)). {
+        eapply trace_connected. apply tr. omega. 
+      }
+      eapply plus_steps. apply H1. apply H2. 
+    } 
+    destruct (f j) as [p js]; destruct p as [jc jl].
+    destruct (f (S j)) as [p sjs]; destruct p as [sjc sjl].  
+    destruct (stack_changes jc sjc jl sjl js sjs H1) as [cond1 | [cond2 | cond3]].
+    ++ simpl. simpl in H. exists lj. subst. reflexivity.
+    ++ simpl. simpl in H. destruct cond2 as [push]. subst. 
+      exists (push :: lj). auto. 
+    ++ simpl. simpl in H. destruct cond3 as [pop].
+      assert(jc = c Skip /\ js = sjs).
+      { eapply pop_skip. rewrite H3 in H1. apply H1. }
+      destruct H4 as [H4 H4'].
+      subst. 
+      destruct lj.
+    * simpl in H1. simpl in H2. simpl in H3.
+      destruct (pop_changes_stacks_identity l2 l2 sjs s2 c2 H2).
+      reflexivity. 
+    * simpl in H3. injection H3. intros. subst. exists lj. reflexivity.
+Qed.
+
+Lemma nil_trace
+        (f: nat -> (instruction * list * state))
+        (c1 c2: instruction) (l1 l2: list) (s1 s2: state):
+    trace f 0 (c1,l1,s1) (c2,l2,s2) ->
+    List.length l1 = List.length l2. 
+Proof.
+  intros. destruct H as [eq1 [eq2 eq3]].
+  rewrite eq1 in eq2. injection eq2. intros. subst. reflexivity.
+Qed.
+
+Lemma linear_traces
+  (f: nat -> (instruction * list * state)) (m j:nat)
+  (c1 c2: instruction * list * state):
+  trace f m c1 c2 -> 0 <= j <=  m ->
+  (exists g m', trace g m' (f j) c2 /\
+           (forall j', j <= j' <=  m -> f j' = g (j' - j)) /\
+           m' + j = m
+  ).
+Proof.
+  intros.
+  induction j.
+  - exists f. exists m. split.
+    + assert(f 0 = c1). { apply H. } rewrite H1. apply H.
+    + split. intros. apply f_equal. omega. omega.
+  - destruct IHj as [g [m' [h1 h2]]]. omega.
+    destruct m.
+    + omega.
+    + destruct m'.
+      * assert(f (S j) ⟹__s* c2).
+        { apply (trace_connected f (S m) c1 c2 H (S j)). omega. }
+        destruct H as [eq1 [eq2 eq3]].
+        destruct h1 as [eq1' [eq2' eq3']].
+        assert(f j ⟹__s f (S j)).
+        { apply eq3. omega. }
+        assert(f j = c2).
+        { rewrite eq1' in eq2'. apply eq2'. }
+        assert(f (S j) ⟹__s+ f (S j)).
+        { eapply plus_right. apply H1. rewrite <- H2. apply H. }
+        exfalso. eapply no_loops. apply H3. reflexivity.
+      * exists (fun n => g (S n)). exists m'. split.
+        ** eapply compute_trace_step. apply h1.
+           destruct H as [eq1 [eq2 eq3]].
+           apply eq3. omega.
+        ** split. intros.        
+           assert(S (j' - S j) = j' - j). omega. rewrite H2.
+           apply h2. omega. omega.
+Qed.
+
+(* pop lemma *)
+Lemma compute_trace
+  (f: nat -> (instruction * list * state)) (m:nat)
+  (c1 c2 a: instruction) (l1 l2: list) (s s': state):
+  trace f m (c1, a::l1 ++ l2,s) (c2,l2,s') ->
+  (exists j s1, 0 <= j <  m /\ f j = (c Skip,a :: l1 ++ l2,s1) ).
+Proof.  
+  intros.
+  induction c1 as [p | c']; intros.
+  - destruct m.
+    + destruct H as [eq1 [eq2 eq3]].
+      rewrite eq1 in eq2. injection eq2. intros.
+      assert(List.length (a :: l1 ++ l2) = List.length l2).
+      { rewrite H0. reflexivity. }
+      simpl in H2. rewrite app_length in H2. omega.
+    + destruct p as [x v].
+      exists 1. exists (update s x v).
+      destruct m.
+      ++ assert(f 0 ⟹__s f 1). { apply H. omega. }
+        assert(f 0 = (i (x, v), a :: l1 ++ l2, s)). { apply H. }
+        assert(f 1 = (c2, l2, s')). { apply H. }
+        assert(f 1 = (c Skip, a :: l1 ++ l2, update s x v)).
+        { rewrite H1 in H0. inversion H0. subst. reflexivity. }
+        rewrite H2 in H3. injection H3. intros.
+        assert(List.length (a :: l1 ++ l2) = List.length l2).
+        { rewrite <- H5. reflexivity. }
+        simpl in H7. rewrite app_length in H7. omega.
+      ++ split. omega. inversion H.
+        assert(f 0 ⟹__s f 1). { apply H1. omega. }
+        rewrite H0 in H2. inversion H2. subst. reflexivity.
+  - generalize dependent c2.
+    generalize dependent a.
+    generalize dependent m.
+    generalize dependent l1.
+    generalize dependent f.
+    generalize dependent s. 
+    induction c'; intros.
+    + destruct m.
+      ++ assert(List.length (a :: l1 ++ l2) = List.length l2).
+        { eapply nil_trace. apply H. }
+        simpl in H0. rewrite app_length in H0. omega.
+      ++ exists 0. exists s. 
+        split. omega.
+        apply H.
+    + destruct m.
+      ++ assert(List.length (a :: l1 ++ l2) = List.length l2).
+        { eapply nil_trace. apply H. }
+        simpl in H0. rewrite app_length in H0. omega.      
+      ++ destruct (IHc'1 s (fun n : nat => f (S n)) (a::l1)
+                  m (c c'2) c2) as [j1 [s1 [h1 h1']]].
+        { eapply compute_trace_step. apply H. apply SComp. }
+        destruct m.        
+        * omega.
+        * assert(f (S j1) ⟹__s f (S (S j1))).
+          { destruct H as [eq1 [eq2 eq3]]. apply eq3. omega.   }
+          assert(f (S (S j1)) = (c c'2,(a :: l1) ++ l2, s1)).
+          { rewrite h1' in H0. inversion H0. subst. reflexivity. }
+          destruct (linear_traces f (S (S m)) (S (S j1))
+          (c (c'1;; c'2), a :: l1 ++ l2, s)
+          (c2, l2, s') H) as [g [m' [h2 [h2' h22]]]]. omega.
+          rewrite H1 in h2.
+          destruct (IHc'2 s1 g l1 m' a c2 h2) as [j3 [s3 [h3 h3']]].
+          exists (j3+(S (S j1))). exists s3.
+          split. omega. rewrite <- h3'.
+          rewrite (h2' (j3 + S (S j1))).
+          assert(j3 + S (S j1) - S (S j1) = j3). omega.
+          rewrite H2. reflexivity. omega.     
+    + assert(f 0 = (c (LET v, t IN c'), a :: l1 ++ l2, s)).
+         { apply H. }                    
+      destruct m.
+     ++ assert(List.length (a :: l1 ++ l2) = List.length l2).
+        { eapply nil_trace. apply H. }
+        simpl in H1. rewrite app_length in H1. omega.     
+     ++ assert(f 0 ⟹__s f 1). { apply H. omega. }
+       assert(trace (fun n : nat => f (S n)) m
+                    (c c', i (v, s v) :: a :: l1 ++ l2,
+                     update s v ⊥) (c2, l2, s')).
+       { eapply compute_trace_step. apply H. apply SLet. }
+       destruct (IHc' (update s v ⊥) (fun n : nat => f (S n))
+                      (a :: l1) m (i (v, s v)) c2 H2)
+         as [j' [s1 [h1 h1']]].       
+       destruct m; try(omega).         
+       assert(f 1 ⟹__s f 2). { apply H. omega. }
+       assert(f 1 = (c c',  i (v, s v) :: a :: l1 ++ l2,
+                     update s v ⊥)).
+       { rewrite H0 in H1. inversion H1. reflexivity. }
+       assert(S j' <= (S (S m))). { omega. }
+       assert(f (S (S m)) = (c2, l2, s')). apply H.                
+       destruct(Nat.eqb_spec (S j') (S (S m))).
+       * exfalso. rewrite e in h1'. rewrite H6 in h1'.
+         injection h1'. intros.
+         assert(List.length l2 =
+                List.length (i (v, s v) :: a :: l1 ++ l2)).
+         { rewrite <- H8. reflexivity. }
+         simpl in H10. omega.
+       * assert(f (S j') ⟹__s f (S (S j'))).
+         { apply H. omega. }
+         assert(f (S (S j')) =  (i (v, s v), (a :: l1) ++ l2, s1)).
+            { rewrite h1' in H7. inversion H7. reflexivity. }
+         destruct(Nat.eqb_spec (S (S j')) (S (S m))).                        ** exfalso. rewrite e in H8. rewrite H6 in H8.
+            injection H8. intros.
+            assert(List.length l2 =
+                List.length (a :: l1 ++ l2)).
+            { rewrite <- H10. reflexivity. }
+            simpl in H12. rewrite app_length in H12. omega.
+         ** assert(f (S (S j')) ⟹__s f (S (S (S j')))).
+            { apply H. omega. }                                                     assert(f (S (S (S j'))) =                                                   (c Skip, a::l1 ++ l2, update s1 v (s v))).
+            { rewrite H8 in H9. inversion H9. reflexivity. }                    destruct(Nat.eqb_spec (S (S (S j'))) (S (S m))).
+            *** exfalso. rewrite e in H10. rewrite H6 in H10.
+                injection H10. intros.
+                assert(List.length l2 =
+                  List.length (a :: l1 ++ l2)).
+                { rewrite <- H12. reflexivity. }
+                simpl in H14. rewrite app_length in H14. omega.
+            *** exists (S (S (S j'))). exists (update s1 v (s v)).
+                split. omega. apply H10.                                            
+   + destruct m. 
+      ++ assert(List.length (a :: l1 ++ l2) = List.length l2).
+        { eapply nil_trace. apply H. }
+        simpl in H0. rewrite app_length in H0. omega.      
+      ++ assert(trace (fun n : nat => f (S n)) m
+            (c Skip, a :: l1 ++ l2,
+             update_list (update s v (aval s e)) (vars e) -__u)
+                     (c2, l2, s')).
+        { eapply compute_trace_step. apply H. apply SAss. }
+        destruct m.
+        * assert(List.length (a :: l1 ++ l2) = List.length l2).
+          { eapply nil_trace. apply H0. }
+          simpl in H1. rewrite app_length in H1. omega.
+        * exists 1. exists (update_list (update s v (aval s e)) (vars e) -__u).
+          split. omega. apply H0.
+Qed.
+
+(* Back to thesis *)
+
+(* Lemma 3.5.1 *)
+Lemma comp_to_skip (c1 c2 : com) (L : list) (s s' : state):
+  (c (c1;;c2),L,s) ⟹__s* (c Skip,L,s') ->
+  (exists (s2 : state),
+      (c c1, c c2 :: L, s) ⟹__s* (c Skip, c c2 :: L,s2) /\
+      ((c Skip, c c2 :: L,s2) ⟹__s (c c2, L, s2)) /\
+       (c c2, L, s2) ⟹__s* (c Skip,L,s')).
+Proof.
+  intros.
+  inversion H; inversion H0. subst.
+  assert(exists f m, trace f m  (c c1, c c2 :: L, s) (c Skip, L, s')).
+  { apply small_trace. apply H1. }
+  destruct H2 as [f [m H']].
+  assert(exists (j : nat) (s1 : state),
+         0 <= j < m /\ f j = (c Skip, (c c2) :: L, s1)).
+  { apply (compute_trace f m (c c1) (c Skip) (c c2) [] L s s').
+    simpl. apply H'. } 
+  destruct H2 as [j [s1 [H2 H2']]].
+  exists s1.
+  destruct (trace_connected f m
+           (c c1, c c2 :: L, s) (c Skip, L, s') H' j) as [eq1 eq2].
+  omega. split.
+  - rewrite H2' in eq2. apply eq2.
+  - split.
+    + apply SLoad.
+    + rewrite H2' in eq1.
+      inversion eq1; subst.
+      ++ assert(List.length (c c2 :: L) = List.length L).
+        { rewrite H5. reflexivity. }
+        simpl in H3. omega.
+      ++ inversion H3. subst. apply H4. 
+Qed.
+
+(* Lemma 3.5.2 *)
+Lemma let_to_skip
+  (c': com) (L : list) (s s' : state) (t: type) (x: string) :
+  (c (LET x , t IN c'),L,s) ⟹__s* (c Skip,L,s') ->
+  (exists (s2 : state),
+      (c (LET x , t IN c'), L, s) ⟹__s*
+      (c Skip, (i (x, s x)) :: L, s2) /\
+      ((c Skip, (i (x, s x)) :: L, s2) ⟹__s (i (x, s x), L,s2)) /\
+       (i (x, s x), L,s2) ⟹__s* (c Skip,L,s')).
+Proof.
+  intros.
+  inversion H; inversion H0. subst.
+  assert(exists f m, trace f m
+          (c c', i (x, s x) :: L, update s x ⊥) (c Skip, L, s')).
+  { apply small_trace. apply H1. }
+  destruct H2 as [f [m H']].
+  assert(exists (j : nat) (s1 : state),
+         0 <= j < m /\ f j = (c Skip, i (x, s x) :: L, s1)).
+  { apply (compute_trace f m (c c') (c Skip)
+                         (i (x, s x)) [] L (update s x ⊥) s').
+    simpl. apply H'. } 
+  destruct H2 as [j [s1 [H2 H2']]].
+  exists s1.
+  destruct (trace_connected f m
+           (c c', i (x, s x) :: L, update s x ⊥)
+           (c Skip, L, s') H' j) as [eq1 eq2].
+  omega. split.
+  - eapply star_step. apply SLet.
+    rewrite H2' in eq2. apply eq2.
+  - split.
+    + apply SLoad.
+    + rewrite H2' in eq1.
+      inversion eq1; subst.
+      ++ assert(List.length (i (x, s x) :: L) = List.length L).
+        { rewrite H5. reflexivity. }
+        simpl in H3. omega.
+      ++ inversion H3. subst. apply H4.
+Qed.
+
+(* Proposition 3.5.3 *)
+
+Lemma between_skips (L : list) (s1 s2 : state):
+  (c Skip, L, s1) ⟹__s* (c Skip, L, s2)  -> s1 = s2.
+Proof.
+  intros.
+  inversion H.
+  - reflexivity.
+  - assert((c Skip, L, s1) ⟹__s+ (c Skip, L, s2)).
+    { eapply plus_steps. apply H0. apply H1. }
+    exfalso.
+    apply (pop_changes_stacks_identity L L s1 s2 (c Skip) H4).
+    reflexivity.
+Qed.
+
+(*
+The effect of a program in memory is not affected by stack content
+*)
+Proposition stack_independence
+  (c': instruction) (l: list) (s s': state) :
+  ((c',l,s) ⟹__s* (c Skip,l,s')) ->
+  (forall l', (c',l',s) ⟹__s* (c Skip,l',s')).
+Proof.
+  intros. 
+  induction c' as [p | c'].
+  - inversion H. subst.
+    inversion H0. subst.
+    assert(s' = update s x v). {
+      rewrite (between_skips l (update s x v) s' H1). reflexivity. }
+    rewrite H2. apply  star_step'. apply SSet.
+  - generalize dependent l.
+    generalize dependent l'. 
+    generalize dependent s.
+    generalize dependent s'.
+    induction c'; intros.
+    + assert(s = s'). eapply between_skips. apply H.
+      rewrite H0. apply star_refl.
+    + destruct (comp_to_skip c'1 c'2 l s s' H) as [s1 [h1 [h2 h3]]].
+      eapply star_step. apply SComp.
+      eapply star_trans. 
+      apply(IHc'1 s1 s ((c c'2) :: l') ((c c'2) :: l) h1).
+      eapply star_step. apply SLoad.
+      apply (IHc'2 s' s1 l' l h3).
+    + destruct (let_to_skip c' l s s' t v H) as [s1 [h1 [h2 h3]]].
+      eapply star_step. apply SLet.
+      eapply star_trans.
+      inversion h1. subst. inversion H0. subst.
+      apply (IHc' s1 (update s v ⊥)
+                  (i (v, s v) :: l') (i (v, s v) :: l) H1).
+      eapply star_step. apply SLoad.
+      eapply star_step. apply SSet.
+      inversion h3. subst. inversion H0. subst.
+      rewrite (between_skips l (update s1 v (s v)) s' H1).
+      apply star_refl.
+    + inversion H. subst.
+      inversion H0. subst.
+      eapply between_skips in H1.
+      eapply star_step. apply SAss.
+      rewrite H1. apply star_refl.
+Qed.
+
+(*
+In a composition, the execution of c1 does not depend 
+on what c2 entails.
+*)
+Lemma sequential_effects
+  (c1 c2: com) (l: list) (s s': state) :
+  ((c c1,l,s) ⟹__s* (c Skip,l,s)) ->
+  ((c (c1 ;; c2),l,s) ⟹__s* (c c2,l,s)).
+Proof.
+  intros.
+  eapply star_step. apply SComp.
+  eapply star_trans.
+  apply (stack_independence (c c1) l s s H (c c2 :: l)).
+  apply star_step'. apply SLoad.
+Qed.
+
+(* Theorem 3.5.5 *)
+Lemma determinism
+  (c' : instruction) (L : list) (s s1 s2 : state) :
+  (c',L,s) ⟹__s* (c Skip,L,s1) ->
+  (c',L,s) ⟹__s* (c Skip,L,s2) ->
+  s1 = s2.
+Proof.
+  intros.
+  destruct c' as [p | c'].
+  - inversion H. inversion H1. subst.
+    inversion H0. inversion H3. subst.
+    rewrite <- (between_skips L (update s x0 v) s1).
+    rewrite <- (between_skips L (update s x0 v) s2).
+    reflexivity. apply H4. apply H2.
+  - generalize dependent L.
+    generalize dependent s1.
+    generalize dependent s2.
+    generalize dependent s. 
+    induction c'; intros. 
+    + rewrite <- (between_skips L s s1).
+      rewrite <- (between_skips L s s2).
+      reflexivity. apply H0. apply H.
+    + inversion H. subst. inversion H1. subst.
+      destruct (comp_to_skip c'1 c'2 L s s1 H) as [s' [h1 [h2 h3]]].
+      destruct (comp_to_skip c'1 c'2 L s s2 H0)
+        as [ss' [h1' [h2' h3']]].
+      remember (IHc'1 s ss' s' (c c'2 :: L) h1 h1') as eq1.
+      subst. 
+      apply (IHc'2 ss' s2 s1 L h3 h3').
+    + destruct (let_to_skip c' L s s1 t v H) as [s' [h1 [h2 h3]]].
+      destruct (let_to_skip c' L s s2 t v H0)
+        as [ss' [h1' [h2' h3']]].
+      inversion h1. inversion H1. subst.
+      inversion h1'. inversion H3. subst.
+      remember (IHc' (update s v ⊥) ss' s'
+                     (i (v, s v) :: L) H2 H4) as eq.
+      subst. 
+      inversion h3. inversion H5. subst. 
+      rewrite <- (between_skips L (update ss' v (s v)) s1).
+      inversion h3'. inversion H7. subst.
+      rewrite <- (between_skips L (update ss' v (s v)) s2).
+      reflexivity. apply H8. apply H6.
+    + inversion H. inversion H1. subst.
+      rewrite <- (between_skips L
+       (update_list (update s v (aval s e)) (vars e) -__u) s1 H2).
+      inversion H0. inversion H3. subst.
+      rewrite <- (between_skips L
+       (update_list (update s v (aval s e)) (vars e) -__u) s2 H4).
+      reflexivity.
+Qed.
