lf/ProofObjects.v
@@ -176,10 +176,12 @@ Print ev_4'''.
 
 Theorem ev_8 : even 8.
 Proof.
-  (* FILL IN HERE *) Admitted.
+  apply ev_SS. apply ev_SS. apply ev_SS.
+  apply ev_SS. apply ev_0.
+Qed.
 
-Definition ev_8' : even 8
-  (* REPLACE THIS LINE WITH ":= _your_definition_ ." *). Admitted.
+Definition ev_8' : even 8 :=
+  ev_SS 6 (ev_SS 4 ev_4).
 (** [] *)
 
 (* ################################################################# *)
@@ -379,10 +381,16 @@ Definition and_comm' P Q : P /\ Q <-> Q /\ P :=
 
 (** **** Exercise: 2 stars, standard, optional (conj_fact)  
 
-    Construct a proof object demonstrating the following proposition. *)
+    Construct a proof object demonstrating the following proposition. *)     
 
-Definition conj_fact : forall P Q R, P /\ Q -> Q /\ R -> P /\ R
-  (* REPLACE THIS LINE WITH ":= _your_definition_ ." *). Admitted.
+Definition conj_fact : forall P Q R, P /\ Q -> Q /\ R -> P /\ R :=
+  fun (P Q R : Prop) (H1: P /\ Q) (H2: Q /\ R) =>
+   match H1 with
+   | conj HP HQ =>
+     match H2 with
+     | conj HQ' HR => conj HP HR
+     end
+   end.
 (** [] *)
 
 (* ================================================================= *)
@@ -411,8 +419,12 @@ End Or.
     Try to write down an explicit proof object for [or_commut] (without
     using [Print] to peek at the ones we already defined!). *)
 
-Definition or_comm : forall P Q, P \/ Q -> Q \/ P
-  (* REPLACE THIS LINE WITH ":= _your_definition_ ." *). Admitted.
+Definition or_comm : forall P Q, P \/ Q -> Q \/ P :=
+  fun (P Q: Prop) (H: P \/ Q) =>
+    match H with
+    | or_introl P  => or_intror P
+    | or_intror Q => or_introl Q
+    end.
 (** [] *)
 
 (* ================================================================= *)
@@ -452,8 +464,8 @@ Definition some_nat_is_even : exists n, even n :=
 
     Complete the definition of the following proof object: *)
 
-Definition ex_ev_Sn : ex (fun n => even (S n))
-  (* REPLACE THIS LINE WITH ":= _your_definition_ ." *). Admitted.
+Definition ex_ev_Sn : ex (fun n => even (S n)) :=
+  ex_intro (fun n => even (S n)) 1 (ev_SS 0 ev_0).
 (** [] *)
 
 (* ================================================================= *)
@@ -545,7 +557,8 @@ Definition singleton : forall (X:Type) (x:X), []++[x] == x::[]  :=
 Lemma equality__leibniz_equality : forall (X : Type) (x y: X),
   x == y -> forall P:X->Prop, P x -> P y.
 Proof.
-(* FILL IN HERE *) Admitted.
+  intros. destruct H. apply H0.
+Qed.
 (** [] *)
 
 (** **** Exercise: 5 stars, standard, optional (leibniz_equality__equality)  
@@ -556,8 +569,9 @@ Proof.
 Lemma leibniz_equality__equality : forall (X : Type) (x y: X),
   (forall P:X->Prop, P x -> P y) -> x == y.
 Proof.
-(* FILL IN HERE *) Admitted.
-
+  intros. 
+  apply ((H (fun z => eq x z)) (eq_refl x)).
+Qed.
 (** [] *)
 
 End MyEquality.
